vale/code/arch/x64/Vale.X64.Memory_Sems.fst
@@ -69,7 +69,7 @@ let same_mem_eq_slices64 b i v k h1 h2 mem1 mem2 =
     UV.length_eq ub
 
 let length_up64 (b:buffer64) (h:vale_heap) (k:nat{k < buffer_length b}) (i:nat{i < 8}) : Lemma
-  (8 * k + i <= DV.length (get_downview b.bsrc)) =
+  (scale8 k + i <= DV.length (get_downview b.bsrc)) =
   let vb = UV.mk_buffer (get_downview b.bsrc) uint64_view in
   UV.length_eq vb
 
@@ -82,11 +82,11 @@ val same_mem_get_heap_val64 (b:buffer64{buffer_writeable b})
                           (mem1:S.machine_heap{IB.correct_down_p (_ih h1) mem1 b})
                           (mem2:S.machine_heap{IB.correct_down_p (_ih h2) mem2 b}) : Lemma
   (requires (Seq.index (buffer_as_seq h1 b) k == Seq.index (buffer_as_seq h2 b) k))
-  (ensures (let ptr = buffer_addr b h1 + 8 * k in
+  (ensures (let ptr = buffer_addr b h1 + scale8 k in
     forall (x:int).{:pattern (mem1.[x])} ptr <= x /\ x < ptr + 8 ==> mem1.[x] == mem2.[x]))
 
 let same_mem_get_heap_val64 b j v k h1 h2 mem1 mem2 =
-  let ptr = buffer_addr b h1 + 8 * k in
+  let ptr = buffer_addr b h1 + scale8 k in
   let addr = buffer_addr b h1 in
   let aux (x:int{ptr <= x /\ x < ptr + 8}) : Lemma (mem1.[x] == mem2.[x]) =
     let i = x - ptr in
@@ -99,13 +99,13 @@ let same_mem_get_heap_val64 b j v k h1 h2 mem1 mem2 =
     let s2 = (Seq.slice (DV.as_seq (IB.hs_of_mem (_ih h2)) db) (k * 8) (k * 8 + 8)) in
     assert (Seq.index s1 i == Seq.index (DV.as_seq (IB.hs_of_mem (_ih h1)) db) (k * 8 + i));
     length_up64 b h1 k i;
-    assert (mem1.[addr+(8 * k + i)] == UInt8.v (Seq.index (DV.as_seq (IB.hs_of_mem (_ih h1)) db) (k * 8 + i)));
+    assert (mem1.[addr+(scale8 k + i)] == UInt8.v (Seq.index (DV.as_seq (IB.hs_of_mem (_ih h1)) db) (k * 8 + i)));
     assert (Seq.index s2 i == Seq.index (DV.as_seq (IB.hs_of_mem (_ih h2)) db) (k * 8 + i));
     length_up64 b h2 k i;
-    assert (mem2.[addr+(8 * k + i)] == UInt8.v (Seq.index (DV.as_seq (IB.hs_of_mem (_ih h2)) db) (k * 8 + i)))
+    assert (mem2.[addr+(scale8 k + i)] == UInt8.v (Seq.index (DV.as_seq (IB.hs_of_mem (_ih h2)) db) (k * 8 + i)))
   in
   Classical.forall_intro aux;
-  assert (forall i. addr + (8 * k + i) == ptr + i)
+  assert (forall i. addr + (scale8 k + i) == ptr + i)
 
 let rec written_buffer_down64_aux1
   (b:buffer64{buffer_writeable b})
@@ -121,12 +121,12 @@ let rec written_buffer_down64_aux1
                  mem1.[j] == mem2.[j])})
   : Lemma
       (ensures (forall j. {:pattern (mem1.[j]) \/ (mem1.[j])}
-                  j >= base /\ j < base + 8 * i ==>
+                  j >= base /\ j < base + scale8 i ==>
                   mem1.[j] == mem2.[j]))
       (decreases %[i-k]) =
     if k >= i then ()
     else begin
-      let ptr = base + 8 * k in
+      let ptr = base + scale8 k in
       same_mem_get_heap_val64 b i v k h h1 mem1 mem2;
       heap_shift mem1 mem2 ptr 8;
       written_buffer_down64_aux1 b i v h base (k+1) h1 mem1 mem2
@@ -143,16 +143,16 @@ let rec written_buffer_down64_aux2
   (mem1:S.machine_heap{IB.correct_down (_ih h) mem1})
   (mem2:S.machine_heap{IB.correct_down (_ih h1) mem2 /\
                (forall j. {:pattern (mem1.[j]) \/ (mem2.[j])}
-                 base + 8 * (i+1) <= j /\ j < base + k * 8 ==>
+                 base + scale8 (i+1) <= j /\ j < base + k * 8 ==>
                  mem1.[j] == mem2.[j])})
   : Lemma
       (ensures (forall j. {:pattern (mem1.[j]) \/ (mem2.[j])}
-                     j >= base + 8 * (i+1) /\ j < base + 8 * n ==>
+                     j >= base + scale8 (i+1) /\ j < base + scale8 n ==>
                      mem1.[j] == mem2.[j]))
       (decreases %[n-k]) =
     if k >= n then ()
     else begin
-      let ptr = base + 8 * k in
+      let ptr = base + scale8 k in
       same_mem_get_heap_val64 b i v k h h1 mem1 mem2;
       heap_shift mem1 mem2 ptr 8;
       written_buffer_down64_aux2 b i v h base n (k+1) h1 mem1 mem2
@@ -168,8 +168,8 @@ let written_buffer_down64 (b:buffer64{buffer_writeable b}) (i:nat{i < buffer_len
           let base = buffer_addr b h in
           let n = buffer_length b in
           forall j. {:pattern (mem1.[j]) \/ (mem2.[j])}
-               (base <= j /\ j < base + 8 * i) \/
-               (base + 8 * (i+1) <= j /\ j < base + 8 * n) ==>
+               (base <= j /\ j < base + scale8 i) \/
+               (base + scale8 (i+1) <= j /\ j < base + scale8 n) ==>
                mem1.[j] == mem2.[j]))
   = let mem1 = I.down_mem (_ih h) in
     let h1 = buffer_write b i v h in
@@ -231,7 +231,7 @@ let store_buffer_down64_mem
         let mem2 = I.down_mem (_ih h1) in
         let base = buffer_addr b h in
         forall (j:int). {:pattern mem1.[j] \/ mem2.[j]}
-          j < base + 8 * i \/ j >= base + 8 * (i+1) ==>
+          j < base + scale8 i \/ j >= base + scale8 (i+1) ==>
           mem1.[j] == mem2.[j]))
   = let mem1 = I.down_mem (_ih h) in
     let h1 = buffer_write b i v h in
@@ -240,7 +240,7 @@ let store_buffer_down64_mem
     let n = buffer_length b in
     let aux (j:int)
       : Lemma
-          (j < base + 8 * i \/ j >= base + 8 * (i+1) ==>
+          (j < base + scale8 i \/ j >= base + scale8 (i+1) ==>
            mem1.[j] == mem2.[j])
       =
       I.addrs_set_lemma_all ();
@@ -269,8 +269,8 @@ let store_buffer_aux_down64_mem (ptr:int) (v:nat64) (h:vale_heap{writeable_mem64
     length_t_eq t b;
     let i = get_addr_in_ptr t (buffer_length b) (buffer_addr b h) ptr 0 in
     store_buffer_write t ptr v h;
-    assert (buffer_addr b h + 8 * i == ptr);
-    assert (buffer_addr b h + 8 * (i+1) == ptr + 8);
+    assert (buffer_addr b h + scale8 i == ptr);
+    assert (buffer_addr b h + scale8 (i+1) == ptr + 8);
     store_buffer_down64_mem b i v h
 
 let store_buffer_aux_down64_mem2 (ptr:int) (v:nat64) (h:vale_heap{writeable_mem64 ptr h})
@@ -290,11 +290,9 @@ let store_buffer_aux_down64_mem2 (ptr:int) (v:nat64) (h:vale_heap{writeable_mem6
     index64_get_heap_val64 h1 b mem2 i
 
 let in_bounds64 (h:vale_heap) (b:buffer64) (i:nat{i < buffer_length b})
-  : Lemma
-      (ensures (forall j. (IB.addrs_of_mem (_ih h)) b + 8 * i <= j  /\
-                     j < (IB.addrs_of_mem (_ih h)) b + 8 * i + 8 ==>
-                     j < (IB.addrs_of_mem (_ih h)) b + DV.length (get_downview b.bsrc)))
-  = length_t_eq (TUInt64) b
+  : Lemma (scale8 i + 8 <= DV.length (get_downview b.bsrc))
+  =
+  length_t_eq TUInt64 b
 
 let bytes_valid64 ptr h =
   reveal_opaque (`%S.valid_addr64) S.valid_addr64;
@@ -320,7 +318,7 @@ val same_mem_get_heap_val128 (b:buffer128)
                           (mem1:S.machine_heap{IB.correct_down_p (_ih h1) mem1 b})
                           (mem2:S.machine_heap{IB.correct_down_p (_ih h2) mem2 b}) : Lemma
   (requires (Seq.index (buffer_as_seq h1 b) k == Seq.index (buffer_as_seq h2 b) k))
-  (ensures (let ptr = buffer_addr b h1 + 16 * k in
+  (ensures (let ptr = buffer_addr b h1 + scale16 k in
     forall i.{:pattern mem1.[i]} i >= ptr /\ i < ptr+16 ==> mem1.[i] == mem2.[i]))
 
 val same_mem_eq_slices128 (b:buffer128)
@@ -348,12 +346,12 @@ let same_mem_eq_slices128 b i v k h1 h2 mem1 mem2 =
     UV.length_eq ub
 
 let length_up128 (b:buffer128) (h:vale_heap) (k:nat{k < buffer_length b}) (i:nat{i < 16}) : Lemma
-  (16 * k + i <= DV.length (get_downview b.bsrc)) =
+  (scale16 k + i <= DV.length (get_downview b.bsrc)) =
   let vb = UV.mk_buffer (get_downview b.bsrc) uint128_view in
   UV.length_eq vb
 
 let same_mem_get_heap_val128 b j v k h1 h2 mem1 mem2 =
-  let ptr = buffer_addr b h1 + 16 * k in
+  let ptr = buffer_addr b h1 + scale16 k in
   let addr = buffer_addr b h1 in
   let aux (i:nat{ptr <= i /\ i < ptr+16}) : Lemma (mem1.[i] == mem2.[i]) =
     let db = get_downview b.bsrc in
@@ -368,15 +366,14 @@ let same_mem_get_heap_val128 b j v k h1 h2 mem1 mem2 =
     assert (mem1.[i] == UInt8.v (Seq.index (DV.as_seq (IB.hs_of_mem (_ih h1)) db) (k * 16 + (i-ptr))));
     assert (Seq.index s2 (i-ptr) == Seq.index (DV.as_seq (IB.hs_of_mem (_ih h2)) db) (k * 16 + (i-ptr)));
     length_up128 b h2 k (i-ptr);
-    assert (mem2.[addr+(16 * k + (i-ptr))] == UInt8.v (Seq.index (DV.as_seq (IB.hs_of_mem (_ih h2)) db) (k * 16 + (i-ptr))));
-    assert (forall i. addr + (16 * k + (i-ptr)) == i)
+    assert (mem2.[addr+(scale16 k + (i-ptr))] == UInt8.v (Seq.index (DV.as_seq (IB.hs_of_mem (_ih h2)) db) (k * 16 + (i-ptr))));
+    assert (forall i. addr + (scale16 k + (i-ptr)) == i)
   in
   Classical.forall_intro aux
 
 let in_bounds128 (h:vale_heap) (b:buffer128) (i:nat{i < buffer_length b}) : Lemma
-  (forall j. j >= (_ih h).IB.addrs b + 16 * i /\
-          j < (_ih h).IB.addrs b + 16 * i + 16 ==>
-          j < (_ih h).IB.addrs b + DV.length (get_downview b.bsrc)) =
+  (scale16 i + 16 <= DV.length (get_downview b.bsrc))
+  =
   length_t_eq TUInt128 b
 
 let bytes_valid128 ptr h =
@@ -415,16 +412,16 @@ let equiv_load_mem64 ptr h =
 
 //let low_lemma_valid_mem64 b i h =
 //  lemma_valid_mem64 b i h;
-//  bytes_valid64 (buffer_addr b h + 8 * i) h
+//  bytes_valid64 (buffer_addr b h + scale8 i) h
 
 //let low_lemma_load_mem64 b i h =
 //  lemma_valid_mem64 b i h;
 //  lemma_load_mem64 b i h;
-//  equiv_load_mem64 (buffer_addr b h + 8 * i) h
+//  equiv_load_mem64 (buffer_addr b h + scale8 i) h
 
 //let same_domain_update64 b i v h =
 //  low_lemma_valid_mem64 b i h;
-//  Vale.Arch.MachineHeap.same_domain_update (buffer_addr b h + 8 * i) v (get_heap h)
+//  Vale.Arch.MachineHeap.same_domain_update (buffer_addr b h + scale8 i) v (get_heap h)
 
 open Vale.X64.BufferViewStore
 
@@ -436,10 +433,10 @@ let low_lemma_store_mem64_aux
   (h:vale_heap{buffer_readable h b /\ buffer_writeable b})
   : Lemma
     (requires IB.correct_down_p (_ih h) heap b)
-    (ensures (let heap' = S.update_heap64 (buffer_addr b h + 8 * i) v heap in
-     let h' = store_mem64 (buffer_addr b h + 8 * i) v h in
+    (ensures (let heap' = S.update_heap64 (buffer_addr b h + scale8 i) v heap in
+     let h' = store_mem64 (buffer_addr b h + scale8 i) v h in
      (_ih h').IB.hs == DV.upd_seq (_ih h).IB.hs (get_downview b.bsrc) (I.get_seq_heap heap' (_ih h).IB.addrs b))) =
-   let ptr = buffer_addr b h + 8 * i in
+   let ptr = buffer_addr b h + scale8 i in
    let heap' = S.update_heap64 ptr v heap in
    let h' = store_mem64 ptr v h in
    lemma_store_mem64 b i v h;
@@ -481,11 +478,11 @@ let valid_state_store_mem64_aux i v h =
 let low_lemma_store_mem64 b i v h =
   lemma_writeable_mem64 b i h;
   lemma_store_mem64 b i v h;
-  valid_state_store_mem64_aux (buffer_addr b h + 8 * i) v h;
+  valid_state_store_mem64_aux (buffer_addr b h + scale8 i) v h;
   let heap = get_heap h in
-  let heap' = S.update_heap64 (buffer_addr b h + 8 * i) v heap in
+  let heap' = S.update_heap64 (buffer_addr b h + scale8 i) v heap in
   low_lemma_store_mem64_aux b heap i v h;
-  Vale.Arch.MachineHeap.frame_update_heap (buffer_addr b h + 8 * i) v heap;
+  Vale.Arch.MachineHeap.frame_update_heap (buffer_addr b h + scale8 i) v heap;
   in_bounds64 h b i;
   I.addrs_set_lemma_all ();
   I.update_buffer_up_mem (_ih h) b heap heap'
@@ -497,12 +494,12 @@ val low_lemma_valid_mem128 (b:buffer128) (i:nat) (h:vale_heap) : Lemma
     buffer_readable h b
   )
   (ensures
-    S.valid_addr128 (buffer_addr b h + 16 * i) (get_heap h)
+    S.valid_addr128 (buffer_addr b h + scale16 i) (get_heap h)
   )
 
 let low_lemma_valid_mem128 b i h =
   lemma_valid_mem128 b i h;
-  bytes_valid128 (buffer_addr b h + 16 * i) h
+  bytes_valid128 (buffer_addr b h + scale16 i) h
 
 val equiv_load_mem128_aux: (ptr:int) -> (h:vale_heap) -> Lemma
   (requires valid_mem128 ptr h)
@@ -528,17 +525,17 @@ val low_lemma_load_mem128 (b:buffer128) (i:nat) (h:vale_heap) : Lemma
     buffer_readable h b
   )
   (ensures
-    S.get_heap_val128 (buffer_addr b h + 16 * i) (get_heap h) == buffer_read b i h
+    S.get_heap_val128 (buffer_addr b h + scale16 i) (get_heap h) == buffer_read b i h
   )
 
 let low_lemma_load_mem128 b i h =
   lemma_valid_mem128 b i h;
   lemma_load_mem128 b i h;
-  equiv_load_mem128_aux (buffer_addr b h + 16 * i) h
+  equiv_load_mem128_aux (buffer_addr b h + scale16 i) h
 
 //let same_domain_update128 b i v h =
 //  low_lemma_valid_mem128 b i h;
-//  Vale.Arch.MachineHeap.same_domain_update128 (buffer_addr b h + 16 * i) v (get_heap h)
+//  Vale.Arch.MachineHeap.same_domain_update128 (buffer_addr b h + scale16 i) v (get_heap h)
 
 let low_lemma_store_mem128_aux
   (b:buffer128)
@@ -548,10 +545,10 @@ let low_lemma_store_mem128_aux
   (h:vale_heap{buffer_readable h b /\ buffer_writeable b})
   : Lemma
     (requires IB.correct_down_p (_ih h) heap b)
-    (ensures (let heap' = S.update_heap128 (buffer_addr b h + 16 * i) v heap in
-     let h' = store_mem128 (buffer_addr b h + 16 * i) v h in
+    (ensures (let heap' = S.update_heap128 (buffer_addr b h + scale16 i) v heap in
+     let h' = store_mem128 (buffer_addr b h + scale16 i) v h in
      (_ih h').IB.hs == DV.upd_seq (_ih h).IB.hs (get_downview b.bsrc) (I.get_seq_heap heap' (_ih h).IB.addrs b))) =
-   let ptr = buffer_addr b h + 16 * i in
+   let ptr = buffer_addr b h + scale16 i in
    let heap' = S.update_heap128 ptr v heap in
    let h' = store_mem128 ptr v h in
    lemma_store_mem128 b i v h;
@@ -585,12 +582,12 @@ let rec written_buffer_down128_aux1
                  mem1.[j] == mem2.[j])})
   : Lemma
       (ensures (forall j. {:pattern (mem1.[j]) \/ (mem1.[j])}
-                  j >= base /\ j < base + 16 * i ==>
+                  j >= base /\ j < base + scale16 i ==>
                   mem1.[j] == mem2.[j]))
       (decreases %[i-k]) =
     if k >= i then ()
     else begin
-      let ptr = base + 16 * k in
+      let ptr = base + scale16 k in
       same_mem_get_heap_val128 b i v k h h1 mem1 mem2;
       heap_shift mem1 mem2 ptr 16;
       written_buffer_down128_aux1 b i v h base (k+1) h1 mem1 mem2
@@ -608,16 +605,16 @@ let rec written_buffer_down128_aux2
   (mem1:S.machine_heap{IB.correct_down (_ih h) mem1})
   (mem2:S.machine_heap{IB.correct_down (_ih h1) mem2 /\
                (forall j. {:pattern (mem1.[j]) \/ (mem2.[j])}
-                 base + 16 * (i+1) <= j /\ j < base + k * 16 ==>
+                 base + scale16 (i+1) <= j /\ j < base + k * 16 ==>
                  mem1.[j] == mem2.[j])})
   : Lemma
       (ensures (forall j. {:pattern (mem1.[j]) \/ (mem2.[j])}
-                     j >= base + 16 * (i+1) /\ j < base + 16 * n ==>
+                     j >= base + scale16 (i+1) /\ j < base + scale16 n ==>
                      mem1.[j] == mem2.[j]))
       (decreases %[n-k]) =
     if k >= n then ()
     else begin
-      let ptr = base + 16 * k in
+      let ptr = base + scale16 k in
       same_mem_get_heap_val128 b i v k h h1 mem1 mem2;
       heap_shift mem1 mem2 ptr 16;
       written_buffer_down128_aux2 b i v h base n (k+1) h1 mem1 mem2
@@ -633,8 +630,8 @@ let written_buffer_down128 (b:buffer128) (i:nat{i < buffer_length b}) (v:quad32)
           let base = buffer_addr b h in
           let n = buffer_length b in
           forall j. {:pattern (mem1.[j]) \/ (mem2.[j])}
-               (base <= j /\ j < base + 16 * i) \/
-               (base + 16 * (i+1) <= j /\ j < base + 16 * n) ==>
+               (base <= j /\ j < base + scale16 i) \/
+               (base + scale16 (i+1) <= j /\ j < base + scale16 n) ==>
                mem1.[j] == mem2.[j]))
   = let mem1 = I.down_mem (_ih h) in
     let h1 = buffer_write b i v h in
@@ -656,7 +653,7 @@ let store_buffer_down128_mem
         let mem2 = I.down_mem (_ih h1) in
         let base = buffer_addr b h in
         forall (j:int). {:pattern mem1.[j] \/ mem2.[j]}
-          j < base + 16 * i \/ j >= base + 16 * (i+1) ==>
+          j < base + scale16 i \/ j >= base + scale16 (i+1) ==>
           mem1.[j] == mem2.[j]))
   = let mem1 = I.down_mem (_ih h) in
     let h1 = buffer_write b i v h in
@@ -665,7 +662,7 @@ let store_buffer_down128_mem
     let n = buffer_length b in
     let aux (j:int)
       : Lemma
-          (j < base + 16 * i \/ j >= base + 16 * (i+1) ==>
+          (j < base + scale16 i \/ j >= base + scale16 (i+1) ==>
            mem1.[j] == mem2.[j])
       =
       I.addrs_set_lemma_all ();
@@ -694,8 +691,8 @@ let store_buffer_aux_down128_mem (ptr:int) (v:quad32) (h:vale_heap{writeable_mem
     length_t_eq t b;
     let i = get_addr_in_ptr t (buffer_length b) (buffer_addr b h) ptr 0 in
     store_buffer_write t ptr v h;
-    assert (buffer_addr b h + 16 * i == ptr);
-    assert (buffer_addr b h + 16 * (i+1) == ptr + 16);
+    assert (buffer_addr b h + scale16 i == ptr);
+    assert (buffer_addr b h + scale16 (i+1) == ptr + 16);
     store_buffer_down128_mem b i v h
 
 let store_buffer_aux_down128_mem2 (ptr:int) (v:quad32) (h:vale_heap{writeable_mem128 ptr h})
@@ -745,12 +742,12 @@ let valid_state_store_mem128_aux i v h =
 let low_lemma_store_mem128 b i v h =
   lemma_valid_mem128 b i h;
   lemma_store_mem128 b i v h;
-  valid_state_store_mem128_aux (buffer_addr b h + 16 * i) v h;
+  valid_state_store_mem128_aux (buffer_addr b h + scale16 i) v h;
   let heap = get_heap h in
-  let heap' = S.update_heap128 (buffer_addr b h + 16 * i) v heap in
-  let h' = store_mem128 (buffer_addr b h + 16 * i) v h in
+  let heap' = S.update_heap128 (buffer_addr b h + scale16 i) v heap in
+  let h' = store_mem128 (buffer_addr b h + scale16 i) v h in
   low_lemma_store_mem128_aux b heap i v h;
-  Vale.Arch.MachineHeap.frame_update_heap128 (buffer_addr b h + 16 * i) v heap;
+  Vale.Arch.MachineHeap.frame_update_heap128 (buffer_addr b h + scale16 i) v heap;
   in_bounds128 h b i;
   I.addrs_set_lemma_all ();
   I.update_buffer_up_mem (_ih h) b heap heap'
@@ -760,8 +757,8 @@ let low_lemma_valid_mem128_64 b i h =
   reveal_opaque (`%S.valid_addr64) S.valid_addr64;
   reveal_opaque (`%S.valid_addr128) S.valid_addr128;
   low_lemma_valid_mem128 b i h;
-  let ptr = buffer_addr b h + 16 * i in
-  assert (buffer_addr b h + 16 * i + 8 = ptr + 8)
+  let ptr = buffer_addr b h + scale16 i in
+  assert (buffer_addr b h + scale16 i + 8 = ptr + 8)
 #pop-options
 
 open Vale.Def.Words.Two_s
@@ -783,8 +780,8 @@ let low_lemma_load_mem128_hi64 b i h =
 
 //let same_domain_update128_64 b i v h =
 //  low_lemma_valid_mem128_64 b i (_ih h);
-//  Vale.Arch.MachineHeap.same_domain_update (buffer_addr b h + 16 * i) v (get_heap h);
-//  Vale.Arch.MachineHeap.same_domain_update (buffer_addr b h + 16 * i + 8) v (get_heap h)
+//  Vale.Arch.MachineHeap.same_domain_update (buffer_addr b h + scale16 i) v (get_heap h);
+//  Vale.Arch.MachineHeap.same_domain_update (buffer_addr b h + scale16 i + 8) v (get_heap h)
 
 open Vale.Def.Types_s
 
@@ -815,7 +812,7 @@ let update_heap128_lo (ptr:int) (v:quad32) (mem:S.machine_heap) : Lemma
   Vale.Arch.MachineHeap.update_heap32_get_heap32 (ptr+12) mem1
 
 let low_lemma_store_mem128_lo64 b i v h =
-  let ptr = buffer_addr b h + 16 * i in
+  let ptr = buffer_addr b h + scale16 i in
   let v128 = buffer_read b i h in
   let v' = insert_nat64 v128 v 0 in
   low_lemma_load_mem128 b i h;
@@ -826,9 +823,11 @@ let low_lemma_store_mem128_lo64 b i v h =
   S.update_heap32_reveal ();
   insert_nat64_reveal ()
 
+#push-options "--z3rlimit 20 --using_facts_from '* -LowStar.Monotonic.Buffer.loc_disjoint_includes_r'"
+#restart-solver
 let low_lemma_store_mem128_hi64 b i v h =
   reveal_opaque (`%S.valid_addr128) S.valid_addr128;
-  let ptr = buffer_addr b h + 16 * i in
+  let ptr = buffer_addr b h + scale16 i in
   let v128 = buffer_read b i h in
   let v' = insert_nat64 v128 v 1 in
   low_lemma_load_mem128 b i h;
@@ -841,3 +840,4 @@ let low_lemma_store_mem128_hi64 b i v h =
   S.update_heap64_reveal ();
   S.update_heap32_reveal ();
   insert_nat64_reveal ()
+#pop-options
