vale/code/arch/x64/Vale.X64.Memory_Sems.fsti
@@ -59,7 +59,7 @@ val equiv_load_mem64 (ptr:int) (m:vale_heap) : Lemma
 //    buffer_readable h b
 //  )
 //  (ensures
-//    S.valid_addr64 (buffer_addr b h + 8 * i) (get_heap h)
+//    S.valid_addr64 (buffer_addr b h + scale8 i) (get_heap h)
 //  )
 
 //val low_lemma_load_mem64 : b:buffer64 -> i:nat -> h:vale_heap -> Lemma
@@ -68,7 +68,7 @@ val equiv_load_mem64 (ptr:int) (m:vale_heap) : Lemma
 //    buffer_readable h b
 //  )
 //  (ensures
-//    S.get_heap_val64 (buffer_addr b h + 8 * i) (get_heap h) == buffer_read b i h
+//    S.get_heap_val64 (buffer_addr b h + scale8 i) (get_heap h) == buffer_read b i h
 //  )
 
 //val same_domain_update64: b:buffer64 -> i:nat -> v:nat64 -> h:vale_heap -> Lemma
@@ -76,7 +76,7 @@ val equiv_load_mem64 (ptr:int) (m:vale_heap) : Lemma
 //    i < Seq.length (buffer_as_seq h b) /\
 //    buffer_readable h b
 //  )
-//  (ensures same_domain h (S.update_heap64 (buffer_addr b h + 8 * i) v (get_heap h)))
+//  (ensures same_domain h (S.update_heap64 (buffer_addr b h + scale8 i) v (get_heap h)))
 
 val low_lemma_store_mem64 (b:buffer64) (i:nat) (v:nat64) (h:vale_heap) : Lemma
   (requires
@@ -85,7 +85,7 @@ val low_lemma_store_mem64 (b:buffer64) (i:nat) (v:nat64) (h:vale_heap) : Lemma
     buffer_writeable b
   )
   (ensures (
-    let m = S.update_heap64 (buffer_addr b h + 8 * i) v (get_heap h) in
+    let m = S.update_heap64 (buffer_addr b h + scale8 i) v (get_heap h) in
     is_machine_heap_update (get_heap h) m /\ upd_heap h m == buffer_write b i v h
   ))
 
@@ -98,7 +98,7 @@ val equiv_load_mem128 (ptr:int) (m:vale_heap) : Lemma
 //    i < Seq.length (buffer_as_seq h b) /\
 //    buffer_readable h b
 //  )
-//  (ensures same_domain h (S.update_heap128 (buffer_addr b h + 16 * i) v (get_heap h)))
+//  (ensures same_domain h (S.update_heap128 (buffer_addr b h + scale16 i) v (get_heap h)))
 
 val low_lemma_store_mem128 (b:buffer128) (i:nat) (v:quad32) (h:vale_heap) : Lemma
   (requires
@@ -107,7 +107,7 @@ val low_lemma_store_mem128 (b:buffer128) (i:nat) (v:quad32) (h:vale_heap) : Lemm
     buffer_writeable b
   )
   (ensures (
-    let m = S.update_heap128 (buffer_addr b h + 16 * i) v (get_heap h) in
+    let m = S.update_heap128 (buffer_addr b h + scale16 i) v (get_heap h) in
     is_machine_heap_update (get_heap h) m /\ upd_heap h m == buffer_write b i v h
   ))
 
@@ -117,8 +117,8 @@ val low_lemma_valid_mem128_64: b:buffer128 -> i:nat -> h:vale_heap -> Lemma
     buffer_readable h b
   )
   (ensures
-    S.valid_addr64 (buffer_addr b h + 16 * i) (get_heap h) /\
-    S.valid_addr64 (buffer_addr b h + 16 * i + 8) (get_heap h)
+    S.valid_addr64 (buffer_addr b h + scale16 i) (get_heap h) /\
+    S.valid_addr64 (buffer_addr b h + scale16 i + 8) (get_heap h)
   )
 
 val low_lemma_load_mem128_lo64 : b:buffer128 -> i:nat -> h:vale_heap -> Lemma
@@ -127,7 +127,7 @@ val low_lemma_load_mem128_lo64 : b:buffer128 -> i:nat -> h:vale_heap -> Lemma
     buffer_readable h b
   )
   (ensures
-    S.get_heap_val64 (buffer_addr b h + 16 * i) (get_heap h) ==
+    S.get_heap_val64 (buffer_addr b h + scale16 i) (get_heap h) ==
       lo64 (buffer_read b i h)
   )
 
@@ -137,7 +137,7 @@ val low_lemma_load_mem128_hi64 : b:buffer128 -> i:nat -> h:vale_heap -> Lemma
     buffer_readable h b
   )
   (ensures
-    S.get_heap_val64 (buffer_addr b h + 16 * i + 8) (get_heap h) ==
+    S.get_heap_val64 (buffer_addr b h + scale16 i + 8) (get_heap h) ==
       hi64 (buffer_read b i h)
   )
 
@@ -147,8 +147,8 @@ val low_lemma_load_mem128_hi64 : b:buffer128 -> i:nat -> h:vale_heap -> Lemma
 //    buffer_readable h b
 //  )
 //  (ensures
-//    same_domain h (S.update_heap64 (buffer_addr b h + 16 * i) v (get_heap h)) /\
-//    same_domain h (S.update_heap64 (buffer_addr b h + 16 * i + 8) v (get_heap h))
+//    same_domain h (S.update_heap64 (buffer_addr b h + scale16 i) v (get_heap h)) /\
+//    same_domain h (S.update_heap64 (buffer_addr b h + scale16 i + 8) v (get_heap h))
 //  )
 
 val low_lemma_store_mem128_lo64 : b:buffer128 -> i:nat-> v:nat64 -> h:vale_heap -> Lemma
@@ -159,7 +159,7 @@ val low_lemma_store_mem128_lo64 : b:buffer128 -> i:nat-> v:nat64 -> h:vale_heap 
   )
   (ensures (
     let v' = insert_nat64 (buffer_read b i h) v 0 in
-    let m = S.update_heap64 (buffer_addr b h + 16 * i) v (get_heap h) in
+    let m = S.update_heap64 (buffer_addr b h + scale16 i) v (get_heap h) in
     is_machine_heap_update (get_heap h) m /\ upd_heap h m == buffer_write b i v' h)
   )
 
@@ -171,6 +171,6 @@ val low_lemma_store_mem128_hi64 : b:buffer128 -> i:nat-> v:nat64 -> h:vale_heap 
   )
   (ensures (
     let v' = insert_nat64 (buffer_read b i h) v 1 in
-    let m = S.update_heap64 (buffer_addr b h + 16 * i + 8) v (get_heap h) in
+    let m = S.update_heap64 (buffer_addr b h + scale16 i + 8) v (get_heap h) in
     is_machine_heap_update (get_heap h) m /\ upd_heap h m == buffer_write b i v' h)
   )
